feat: FLTS

Cslib/Computability/Automata/Deterministic/DA.lean
@@ -4,7 +4,8 @@ Released under Apache 2.0 license as described in the file LICENSE.
 Authors: Fabrizio Montesi
 -/
 
-import Cslib.Init
+import Cslib.Computability.Automata.Acceptor
+import Cslib.Foundations.Semantics.LTS.FLTS
 
 /-! # Deterministic Automaton
 
@@ -13,26 +14,24 @@ A Deterministic Automaton (DA) is an automaton defined by a transition function.
 
 namespace Cslib.Automata
 
-structure DA (State : Type _) (Symbol : Type _) where
+structure DA (State : Type _) (Symbol : Type _) extends FLTS State Symbol where
   /-- The initial state of the automaton. -/
   start : State
-  /-- The transition function of the automaton. -/
-  tr : State → Symbol → State
+  /-- The accept states of the automaton. -/
+  accept : Set State
 
 namespace DA
 
 variable {State : Type _} {Symbol : Type _}
 
-/-- Extended transition function.
+/-- Returns the acceptor that matches exactly the sequence of symbols in a string.
+That is, a string is accepted if the multistep transition function of the `DA` maps the start state
+and the string to an accept state.
 
-Implementation note: compared to [Hopcroft2006], the definition consumes the input list of symbols
-from the left (instead of the right), in order to match the way lists are constructed.
--/
+This is the standard string recognition performed by DFAs in the literature. -/
 @[scoped grind =]
-def mtr (da : DA State Symbol) (s : State) (xs : List Symbol) := xs.foldl da.tr s
-
-@[scoped grind =]
-theorem mtr_nil_eq {da : DA State Symbol} {s : State} : da.mtr s [] = s := rfl
+def acceptor (da : DA State Symbol) : Acceptor Symbol where
+  Accepts (xs : List Symbol) := da.mtr da.start xs ∈ da.accept
 
 end DA
 
