Cslib/Computability/Automata/DAToNA.lean
@@ -1,0 +1,47 @@
+/-
+Copyright (c) 2025 Fabrizio Montesi. All rights reserved.
+Released under Apache 2.0 license as described in the file LICENSE.
+Authors: Fabrizio Montesi
+-/
+
+import Cslib.Computability.Automata.Deterministic.ExactAcceptor
+import Cslib.Computability.Automata.Nondeterministic.ExactAcceptor
+
+/-! # Translation of a `DA.ExactAcceptor` into an `NA.ExactAcceptor`.
+
+This is the general version of the standard translation of DFAs into NFAs. -/
+
+namespace Cslib.Automata.DA
+
+variable {State : Type _} {Symbol : Type _}
+
+section NA
+
+-- /-- `DA` is a special case of `NA`. -/
+-- @[scoped grind =]
+-- def toNA (da : DA State Symbol) : NA State Symbol where
+--   start := {da.start}
+--   Tr := fun s1 μ s2 => da.tr s1 μ = s2
+
+-- @[scoped grind =]
+-- lemma toNA_start {da : DA State Symbol} : da.toNA.start = {da.start} := rfl
+
+-- instance : Coe (DA State Symbol) (NA State Symbol) where
+--   coe := toNA
+
+
+/-- The `NFA` constructed from a `DFA` has the same language. -/
+@[scoped grind =]
+theorem toNA_exactAcceptor_language_eq {da : DA State Symbol} {acc : Set State} :
+    (da.exactAcceptor acc).language = (da.toNA.exactAcceptor acc).language := by
+  ext xs
+  apply Iff.intro <;> intro h
+  case mp =>
+    simp_all [NA.exactAcceptor, DA.exactAcceptor, Acceptor.language]
+
+    open NA Acceptor DA in grind
+  refine ⟨?_, fun _ => ⟨da.start, ?_⟩⟩ <;> open NA Acceptor in grind
+
+end NA
+
+end Cslib.Automata.DA
