Cslib/Computability/Automata/NAToDA.lean
@@ -1,0 +1,45 @@
+/-
+Copyright (c) 2025 Fabrizio Montesi. All rights reserved.
+Released under Apache 2.0 license as described in the file LICENSE.
+Authors: Fabrizio Montesi
+-/
+
+import Cslib.Computability.Automata.Deterministic.DA
+import Cslib.Computability.Automata.Nondeterministic.NA
+import Cslib.Foundations.Semantics.LTS.LTSToFLTS
+
+/-! # Translation of NFA into DFA (subset construction) -/
+
+namespace Cslib.Automata.NA
+
+variable {State : Type _} {Symbol : Type _}
+
+section SubsetConstruction
+
+/-- Converts an `NA` into a `DA` using the subset construction. -/
+@[scoped grind =]
+def toDA (na : NA State Symbol) : DA (Set State) Symbol := {
+  start := na.start
+  accept := { S | ∃ s ∈ S, s ∈ na.accept }
+  tr := na.toFLTS.tr
+}
+
+/-- The `DA` constructed from an `NA` has the same language. -/
+@[scoped grind =]
+theorem toDA_language_eq {na : NA State Symbol} :
+  na.toDA.acceptor.language = na.acceptor.language := by
+  ext xs
+  -- simp [toDA, NA.acceptor, DA.acceptor]
+  rw [Acceptor.mem_language]
+  rw [Acceptor.mem_language]
+  -- simp [LTS.toFLTS]
+  #adaptation_note
+  /--
+  Moving from `nightly-2025-09-15` to `nightly-2025-10-19` required
+  increasing the number of allowed splits.
+  -/
+  open DA NA Acceptor FLTS LTS in grind (splits := 12)
+
+end SubsetConstruction
+
+end Cslib.Automata.NA
